more rewriting.

doc/simple/coq/Exists.v
@@ -10,99 +10,121 @@ Require Import LibReflect.
 
 Definition cpltctxsubst_exists_def := forall G e,
     AWf G ->
-    AWTerm G e ->
-    CompleteCtx G ->
-    exists t, ACpltCtxSubst G e t
-.
-
-Definition cpltctxtsubst_exists_def := forall G e,
-    AWf G ->
     AWTermT G e ->
     CompleteCtx G ->
-    exists t, ACpltCtxTSubst G e t
+    exists t, ACpltCtxSubst G e t
 .
 
 (* admitted lemma with issue about quantification *)
 
 Lemma lam_solve: forall G x e t,
     AWf (G & x ~ AC_Var) ->
-    ACpltCtxSubst (G & x ~ AC_Var) (e @ x) t ->
-    exists d, ACpltCtxSubst G (AE_Lam e) d.
+    ACpltCtxSubst (G & x ~ AC_Var) (AT_Expr (e @ x)) t ->
+    exists d, ACpltCtxSubst G (AT_Expr (AE_Lam e)) d.
 Admitted.
 
 Lemma pi_solve: forall G x e1 e2 t1 t2,
     AWf (G & x ~ AC_Var) ->
     ACpltCtxSubst G e1 t1 ->
-    ACpltCtxSubst (G & x ~ AC_Var) (e2 @ x) t2 ->
-    exists d, ACpltCtxSubst G (AE_Pi e1 e2) d.
-Admitted.
-
-Lemma let_solve: forall G x e1 e2 t1 t2,
-    AWf (G & x ~ AC_Var) ->
-    ACpltCtxSubst G e1 t1 ->
-    ACpltCtxSubst (G & x ~ AC_Var) (e2 @ x) t2 ->
-    exists d, ACpltCtxSubst G (AE_Let e1 e2) d.
+    ACpltCtxSubst (G & x ~ AC_Var) (e2 @' x) t2 ->
+    exists d, ACpltCtxSubst G (AT_Expr (AE_Pi e1 e2)) d.
 Admitted.
 
 Lemma forall_solve: forall G x e t,
-    AWf (G & x ~ AC_Var) ->
-    ACpltCtxTSubst (G & x ~ AC_Typ AE_Star) (e @' x) t ->
-    exists d, ACpltCtxTSubst G (AT_Forall e) d.
+    AWf (G & x ~ AC_TVar) ->
+    ACpltCtxSubst (G & x ~ AC_TVar) (e @#' x) t ->
+    exists d, ACpltCtxSubst G (AT_Expr (AE_Forall e)) d.
 Admitted.
 
 (* another form of awterm, which does not care about bound variables *)
 
-Inductive AWTermA : ACtx -> AExpr -> Prop :=
-  | AWTermA_Var : forall G x, binds x AC_Var G -> AWTermA G (AE_FVar x)
-  | AWTermA_BVar : forall G x, AWTermA G (AE_BVar x)
-  | AWTermA_TypVar : forall G x t, binds x (AC_Typ t) G -> AWTermA G (AE_FVar x)
-  | AWTermA_LetVar : forall G x t e, binds x (AC_Bnd t e) G -> AWTermA G (AE_FVar x)
-  | AWTermA_EVar : forall G a, binds a AC_Unsolved_EVar G -> AWTermA G (AE_EVar a)
-  | AWTermA_Solved_EVar : forall G a t, binds a (AC_Solved_EVar t) G -> AWTermA G (AE_EVar a)
-  | AWTermA_Star: forall G, AWTermA G AE_Star
-  | AWTermA_App: forall e1 e2 G, AWTermA G e1 -> AWTermA G e2 -> AWTermA G (AE_App e1 e2)
-  | AWTermA_Lam: forall e G , AWTermA G e  -> AWTermA G (AE_Lam e)
-  | AWTermA_Pi: forall t1 t2 G, AWTermA G t1 -> AWTermA G t2 -> AWTermA G (AE_Pi t1 t2)
-  | AWTermA_Let: forall e1 e2 G, AWTermA G e1 -> AWTermA G e2 -> AWTermA G (AE_Let e1 e2)
-  | AWTermA_CastUp : forall e G, AWTermA G e -> AWTermA G (AE_CastUp e)
-  | AWTermA_CastDn : forall e G, AWTermA G e -> AWTermA G (AE_CastDn e)
-  | AWTermA_Ann: forall e1 e2 G, AWTermA G e1 -> AWTermA G e2 -> AWTermA G (AE_Ann e1 e2)
+Inductive AWTermA : ACtx -> AType -> Prop :=
+  | AWTermA_Var : forall G x, binds x AC_Var G -> AWTermA G (AT_Expr (AE_FVar x))
+  | AWTermA_BVar : forall G x, AWTermA G (AT_Expr (AE_BVar x))
+  | AWTermA_TypVar : forall G x t, binds x (AC_Typ t) G -> AWTermA G (AT_Expr (AE_FVar x))
+  | AWTermA_TFVar : forall G a, binds a AC_TVar G -> AWTermA G (AT_TFVar a)
+  | AWTermA_TBVar : forall G x, AWTermA G (AT_TBVar x)
+  | AWTermA_EVar : forall G a, binds a AC_Unsolved_EVar G -> AWTermA G (AT_EVar a)
+  | AWTermA_Solved_EVar : forall G a t, binds a (AC_Solved_EVar t) G -> AWTermA G (AT_EVar a)
+  | AWTermA_Star: forall G, AWTermA G (AT_Expr AE_Star)
+  | AWTermA_App: forall e1 e2 G, AWTermA G (AT_Expr e1) -> AWTermA G (AT_Expr e2) -> AWTermA G (AT_Expr (AE_App e1 e2))
+  | AWTermA_Lam: forall e G , AWTermA G (AT_Expr e)  -> AWTermA G (AT_Expr (AE_Lam e))
+  | AWTermA_Pi: forall t1 t2 G, AWTermA G t1 -> AWTermA G t2 -> AWTermA G (AT_Expr (AE_Pi t1 t2))
+  | AWTermA_CastUp : forall e G, AWTermA G (AT_Expr e) -> AWTermA G (AT_Expr (AE_CastUp e))
+  | AWTermA_CastDn : forall e G, AWTermA G (AT_Expr e) -> AWTermA G (AT_Expr (AE_CastDn e))
+  | AWTermA_Ann: forall e1 e2 G, AWTermA G (AT_Expr e1) -> AWTermA G e2 -> AWTermA G (AT_Expr (AE_Ann e1 e2))
+  | AWTermA_Forall: forall e G, AWTermA G e -> AWTermA G (AT_Expr (AE_Forall e))
 .
 
 (* helper lemmas *)
 Hint Constructors AWTermA ACpltCtxSubst.
 Hint Resolve awf_is_ok AWf_left complete_part_left complete_part_right.
 Lemma awterma_open: forall G k u e,
-    AWTermA G (AOpenRec k u e) ->
+    AWTermA G (AT_Expr (AOpenRec k u e)) ->
+    AWTermA G (AT_Expr e)
+with awterma_opent: forall G k u e,
+    AWTermA G (AOpenTypRec k u e) ->
     AWTermA G e.
 Proof.
-  introv wt. gen k u. induction e; intros; simpls; auto_star;
-  try(inversion wt; subst; auto_star).
+  introv wt. gen k u. induction e; intros; simpls.
+  case_nat*. assumption. assumption.
+  inversion wt; subst. apply AWTermA_App. apply* IHe1. apply* IHe2.
+  inversion wt; subst. apply AWTermA_Lam. apply* IHe.
+  inversion wt; subst. apply AWTermA_Pi. apply* awterma_opent. apply* awterma_opent.
+  inversion wt; subst. apply AWTermA_CastUp. apply* IHe.
+  inversion wt; subst. apply AWTermA_CastDn. apply* IHe.
+  inversion wt; subst. apply AWTermA_Ann. apply* IHe. apply* awterma_opent.
+  inversion wt; subst. apply AWTermA_Forall. apply* awterma_opent.
+Proof.
+  introv wt. gen k u. induction e; intros; simpls.
+  assumption. assumption. assumption.
+  apply* awterma_open.
+Qed.
+
+Lemma awterma_topen: forall G k u e,
+    AWTermA G (AT_Expr (ATOpenRec k u e)) ->
+    AWTermA G (AT_Expr e)
+with awterma_topent: forall G k u e,
+    AWTermA G (ATOpenTypRec k u e) ->
+    AWTermA G e.
+Proof.
+  introv wt. gen k u. induction e; intros; simpls.
+  assumption. assumption. assumption.
+  inversion wt; subst. apply AWTermA_App. apply* IHe1. apply* IHe2.
+  inversion wt; subst. apply AWTermA_Lam. apply* IHe.
+  inversion wt; subst. apply AWTermA_Pi. apply* awterma_topent. apply* awterma_topent.
+  inversion wt; subst. apply AWTermA_CastUp. apply* IHe.
+  inversion wt; subst. apply AWTermA_CastDn. apply* IHe.
+  inversion wt; subst. apply AWTermA_Ann. apply* IHe. apply* awterma_topent.
+  inversion wt; subst. apply AWTermA_Forall. apply* awterma_topent.
+Proof.
+  introv wt. gen k u. induction e; intros; simpls.
+  case_nat*. assumption. assumption.
+  apply* awterma_topen.
 Qed.
 
 Lemma awterma_remove: forall G H e y v,
     AWTermA (G & y ~ v & H) e ->
-    y \notin AFv e ->
+    y \notin ATFv e ->
     AWTermA (G & H) e.
 Proof.
   introv wt notin. gen_eq I: (G & y ~ v & H).
   gen H. induction wt; introv hh; auto_star.
   simpl in notin. rewrite hh in H. apply AWTermA_Var. apply* binds_subst.
   simpl in notin. rewrite hh in H. apply* AWTermA_TypVar. apply* binds_subst.
-  simpl in notin. rewrite hh in H. apply* AWTermA_LetVar. apply* binds_subst.
+  simpl in notin. rewrite hh in H. apply* AWTermA_TFVar. apply* binds_subst.
   simpl in notin. rewrite hh in H. apply* AWTermA_EVar. apply* binds_subst.
   simpl in notin. rewrite hh in H. apply* AWTermA_Solved_EVar. apply* binds_subst.
 
-  simpl in notin. apply AWTermA_App. apply* IHwt1. apply* IHwt2.
+  simpl in notin. apply AWTermA_App. apply* IHwt1. simpls*. apply* IHwt2. simpls*.
 
   simpl in notin. apply AWTermA_Pi. apply* IHwt1. apply* IHwt2.
-  simpl in notin. apply AWTermA_Let. apply* IHwt1. apply* IHwt2.
-  simpl in notin. apply AWTermA_Ann. apply* IHwt1. apply* IHwt2.
+  simpl in notin. apply AWTermA_Ann. apply* IHwt1. simpls*. apply* IHwt2.
 Qed.
 
 Lemma awterma_remove_empty: forall G e y v,
     AWTermA (G & y ~ v) e ->
-    y \notin AFv e ->
+    y \notin ATFv e ->
     AWTermA G e.
 Proof.
   intros. assert (AWTermA (G & y ~ v & empty) e). rewrite* concat_empty_r.
@@ -113,16 +135,16 @@ Qed.
 (* one important one, changes from awterm to awterma *)
 
 Theorem awterm_is_awterma: forall G e,
-    AWTerm G e ->
+    AWTermT G e ->
     AWTermA G e.
 Proof.
   introv wt. induction wt; auto_star.
-  pick_fresh y. assert (AWTermA (G & y ~ AC_Var) (e @ y)).
-  apply H0. auto_star. apply awterma_open in H1. apply awterma_remove_empty in H1. constructor*. auto_star.
-  constructor*. pick_fresh y. assert (AWTermA (G & y ~ AC_Var) (t2 @ y)).
-  apply H0. auto_star. apply awterma_open in H1. apply awterma_remove_empty in H1. auto_star. auto_star.
-  constructor*. pick_fresh y. assert (AWTermA (G & y ~ AC_Var) (e2 @ y)).
-  apply H0. auto_star. apply awterma_open in H1. apply awterma_remove_empty in H1. auto_star. auto_star.
+  pick_fresh y. assert (AWTermA (G & y ~ AC_Var) (AT_Expr (e @ y))).
+  apply H0. auto_star. apply awterma_open in H1. apply awterma_remove_empty in H1. constructor*. simpls*.
+  constructor*. pick_fresh y. assert (AWTermA (G & y ~ AC_Var) (t2 @' y)).
+  apply H0. auto_star. apply awterma_opent in H1. apply awterma_remove_empty in H1. auto_star. auto_star.
+  constructor*. pick_fresh y. assert (AWTermA (G & y ~ AC_TVar) (s @#' y)).
+  apply H0. auto_star. apply awterma_topent in H1. apply awterma_remove_empty in H1. auto_star. auto_star.
 Qed.
 
 (* a definition about length of a expression.
@@ -130,136 +152,243 @@ Qed.
 ( there are many meaningless definition,
 ( which ends with `I` *)
 
-Inductive ALen : ACtx -> AExpr -> nat -> Prop :=
-| ALen_BVar: forall G i, ALen G (AE_BVar i) 1
-| ALen_Var: forall G x, binds x AC_Var G -> ALen G (AE_FVar x) 1
-| ALen_TypVar: forall G x t, binds x (AC_Typ t) G -> ALen G (AE_FVar x) 1
-| ALen_LetVar : forall G x t e i, binds x (AC_Bnd t e) G -> ALen G e i -> ALen G (AE_FVar x) (i + 1)
-| ALen_Var_I1 : forall G x, binds x AC_Unsolved_EVar G -> ALen G (AE_FVar x) 1
-| ALen_Var_I2 : forall G x t, binds x (AC_Solved_EVar t) G -> ALen G (AE_FVar x) 1
-| ALen_Var_I : forall G x, x # G -> ALen G (AE_FVar x) 1
-| ALen_EVar : forall G a, binds a AC_Unsolved_EVar G -> ALen G (AE_EVar a) 1
-| ALen_EVar_I1: forall G x, binds x AC_Var G -> ALen G (AE_EVar x) 1
-| ALen_EVar_I2: forall G x t, binds x (AC_Typ t) G -> ALen G (AE_EVar x) 1
-| ALen_EVar_I3: forall G x t e, binds x (AC_Bnd t e) G -> ALen G (AE_EVar x) 1
-| ALen_Solved_EVar: forall G1 G2 a t i, ok (G1 & a ~ AC_Solved_EVar t & G2) -> ALen G1 t i -> ALen (G1 & a ~ AC_Solved_EVar t & G2) (AE_EVar a) (i + 1)
-| ALen_EVar_I : forall G a, a # G -> ALen G (AE_EVar a) 1
-| ALen_Star: forall G, ALen G (AE_Star) 1
-| ALen_App: forall e1 e2 G i1 i2, ALen G e1 i1 -> ALen G e2 i2 -> ALen G (AE_App e1 e2) (i1 + i2 + 1)
-| ALen_Lam: forall e G i, ALen G e i -> ALen G (AE_Lam e) (i + 1)
-| ALen_Pi: forall e1 e2 G i1 i2, ALen G e1 i1 -> ALen G e2 i2 -> ALen G (AE_Pi e1 e2) (i1 + i2 + 1)
-| ALen_Let: forall e1 e2 G i1 i2, ALen G e1 i1 -> ALen G e2 i2 -> ALen G (AE_Let e1 e2) (i1 + i2 + 1)
-| ALen_CastUp:  forall e G i, ALen G e i -> ALen G (AE_CastUp e) (i + 1)
-| ALen_CastDn:  forall e G i, ALen G e i -> ALen G (AE_CastDn e) (i + 1)
-| ALen_Ann: forall e1 e2 G i1 i2, ALen G e1 i1 -> ALen G e2 i2 -> ALen G (AE_Ann e1 e2) (i1 + i2 + 1).
+Inductive ALen : ACtx -> AType -> nat -> Prop :=
+| ALen_Var: forall G x, binds x AC_Var G -> ALen G (AT_Expr (AE_FVar x)) 1
+| ALen_BVar: forall G i, ALen G (AT_Expr (AE_BVar i)) 1
+| ALen_TypVar: forall G x t, binds x (AC_Typ t) G -> ALen G (AT_Expr (AE_FVar x)) 1
+| ALen_Var_I1 : forall G x, binds x AC_Unsolved_EVar G -> ALen G (AT_Expr (AE_FVar x)) 1
+| ALen_Var_I2 : forall G x t, binds x (AC_Solved_EVar t) G -> ALen G (AT_Expr (AE_FVar x)) 1
+| ALen_Var_I3 : forall G x, binds x AC_TVar G -> ALen G (AT_Expr (AE_FVar x)) 1
+| ALen_Var_I : forall G x, x # G -> ALen G (AT_Expr (AE_FVar x)) 1
+| ALen_EVar : forall G a, binds a AC_Unsolved_EVar G -> ALen G (AT_EVar a) 1
+| ALen_Solved_EVar: forall G1 G2 a t i,
+    ok (G1 & a ~ AC_Solved_EVar t & G2) ->
+    ALen G1 t i -> ALen (G1 & a ~ AC_Solved_EVar t & G2) (AT_EVar a) (i + 1)
+| ALen_EVar_I1: forall G x, binds x AC_Var G -> ALen G (AT_EVar x) 1
+| ALen_EVar_I2: forall G x t, binds x (AC_Typ t) G -> ALen G (AT_EVar x) 1
+| ALen_EVar_I3: forall G x, binds x (AC_TVar) G -> ALen G (AT_EVar x) 1
+| ALen_EVar_I : forall G a, a # G -> ALen G (AT_EVar a) 1
+| ALen_TBVar: forall G i, ALen G (AT_TBVar i) 1
+| ALen_TFVar: forall G a, binds a AC_TVar G -> ALen G (AT_TFVar a) 1
+| ALen_TFVar_I1: forall G a, binds a AC_Var G -> ALen G (AT_TFVar a) 1
+| ALen_TFVar_I2: forall G a t, binds a (AC_Typ t) G -> ALen G (AT_TFVar a) 1
+| ALen_TFVar_I3: forall G a, binds a AC_Unsolved_EVar G -> ALen G (AT_TFVar a) 1
+| ALen_TFVar_I4: forall G a t, binds a (AC_Solved_EVar t) G -> ALen G (AT_TFVar a) 1
+| ALen_TFVar_I: forall G a, a # G -> ALen G (AT_TFVar a) 1
+| ALen_Star: forall G, ALen G (AT_Expr AE_Star) 1
+| ALen_App: forall e1 e2 G i1 i2, ALen G (AT_Expr e1) i1 -> ALen G (AT_Expr e2) i2 -> ALen G (AT_Expr (AE_App e1 e2)) (i1 + i2 + 1)
+| ALen_Lam: forall e G i, ALen G (AT_Expr e) i -> ALen G (AT_Expr (AE_Lam e)) (i + 1)
+| ALen_Pi: forall e1 e2 G i1 i2, ALen G e1 i1 -> ALen G e2 i2 -> ALen G (AT_Expr (AE_Pi e1 e2)) (i1 + i2 + 1)
+| ALen_CastUp:  forall e G i, ALen G (AT_Expr e) i -> ALen G (AT_Expr (AE_CastUp e)) (i + 1)
+| ALen_CastDn:  forall e G i, ALen G (AT_Expr e) i -> ALen G (AT_Expr (AE_CastDn e)) (i + 1)
+| ALen_Ann: forall e1 e2 G i1 i2, ALen G (AT_Expr e1) i1 -> ALen G e2 i2 -> ALen G (AT_Expr (AE_Ann e1 e2)) (i1 + i2 + 1)
+| ALen_Forall: forall e G i, ALen G e i -> ALen G (AT_Expr (AE_Forall e)) (i + 1).
 
 Hint Constructors ALen.
 
 (* some lemmas about alen *)
 
-Lemma alen_add_var': forall G e i y m,
+Lemma alen_add_var_expr: forall G i y e,
+    ALen G (AT_Expr e) i ->
+    ok (G & y ~ AC_Var) ->
+    ALen (G & y ~ AC_Var) (AT_Expr e) i
+with alen_add_var: forall G i y e,
     ALen G e i ->
-    i < m ->
     ok (G & y ~ AC_Var) ->
     ALen (G & y ~ AC_Var) e i.
 Proof.
-  introv. gen G e i y. induction m.
-  introv len less okg.
-  inversion less.
+  introv len okg.
+  gen i. induction e; introv len.
 
-  introv len less okg.
-  gen i. induction e; introv len less.
   inversion len; subst. apply ALen_BVar.
+
   inversion len; subst.
   assert (v<>y). intros neq. subst. apply ok_push_inv in okg. destruct okg as [_ okg]. false binds_fresh_inv H1 okg.
   apply ALen_Var. apply* binds_concat_left.
-
   assert (v<>y). intros neq. subst. apply ok_push_inv in okg. destruct okg as [_ okg]. false binds_fresh_inv H1 okg.
   apply ALen_TypVar with t. apply* binds_concat_left.
-
-  assert (v<>y). intros neq. subst. apply ok_push_inv in okg. destruct okg as [_ okg]. false binds_fresh_inv H0 okg.
-  apply ALen_LetVar with t e. apply* binds_concat_left.
-  apply* IHm. Omega.omega.
-
   assert (v<>y). intros neq. subst. apply ok_push_inv in okg. destruct okg as [_ okg]. false binds_fresh_inv H1 okg.
   apply ALen_Var_I1. apply* binds_concat_left.
-
   assert (v<>y). intros neq. subst. apply ok_push_inv in okg. destruct okg as [_ okg]. false binds_fresh_inv H1 okg.
   apply ALen_Var_I2 with t. apply* binds_concat_left.
-
+  assert (v<>y). intros neq. subst. apply ok_push_inv in okg. destruct okg as [_ okg]. false binds_fresh_inv H1 okg.
+  apply ALen_Var_I3. apply* binds_concat_left.
   destruct (eq_var_dec v y). subst.
   apply ALen_Var. apply* binds_push_eq.
-
   apply ALen_Var_I. auto_star.
 
-  inversion len; subst. apply ALen_EVar.
-  assert (v<>y). intros neq. subst. apply ok_push_inv in okg. destruct okg as [_ okg]. false binds_fresh_inv H1 okg.
-  apply* binds_concat_left.
+  inversion len; subst. apply ALen_Star.
+  inversion len; subst. apply ALen_App.
+  apply* IHe1.
+  apply* IHe2.
 
-  assert (v<>y). intros neq. subst. apply ok_push_inv in okg. destruct okg as [_ okg]. false binds_fresh_inv H1 okg.
-  apply ALen_EVar_I1. apply* binds_concat_left.
+  inversion len; subst. apply ALen_Lam.
+  apply* IHe.
 
-  assert (v<>y). intros neq. subst. apply ok_push_inv in okg. destruct okg as [_ okg]. false binds_fresh_inv H1 okg.
-  apply ALen_EVar_I2 with t. apply* binds_concat_left.
+  inversion len; subst. apply ALen_Pi.
+  apply* alen_add_var.
+  apply* alen_add_var.
 
-  assert (v<>y). intros neq. subst. apply ok_push_inv in okg. destruct okg as [_ okg]. false binds_fresh_inv H1 okg.
-  apply ALen_EVar_I3 with t e. apply* binds_concat_left.
+  inversion len; subst. apply ALen_CastUp.
+  apply* IHe.
 
+  inversion len; subst. apply ALen_CastDn.
+  apply* IHe.
+
+  inversion len; subst. apply ALen_Ann.
+  apply* IHe.
+  apply* alen_add_var.
+
+  inversion len; subst. apply ALen_Forall.
+  apply* alen_add_var.
+Proof.
+  introv len okg.
+  gen i. induction e; introv len.
+
+  inversion len; subst. apply ALen_TBVar.
+
+  inversion len; subst.
+  assert (v<>y). intros neq. subst. apply ok_push_inv in okg. destruct okg as [_ okg]. false binds_fresh_inv H1 okg.
+  apply ALen_TFVar. apply* binds_concat_left.
+  assert (v<>y). intros neq. subst. apply ok_push_inv in okg. destruct okg as [_ okg]. false binds_fresh_inv H1 okg.
+  apply ALen_TFVar_I1. apply* binds_concat_left.
+  assert (v<>y). intros neq. subst. apply ok_push_inv in okg. destruct okg as [_ okg]. false binds_fresh_inv H1 okg.
+  apply ALen_TFVar_I2 with t. apply* binds_concat_left.
+  assert (v<>y). intros neq. subst. apply ok_push_inv in okg. destruct okg as [_ okg]. false binds_fresh_inv H1 okg.
+  apply ALen_TFVar_I3. apply* binds_concat_left.
+  assert (v<>y). intros neq. subst. apply ok_push_inv in okg. destruct okg as [_ okg]. false binds_fresh_inv H1 okg.
+  apply ALen_TFVar_I4 with t. apply* binds_concat_left.
+  destruct (eq_var_dec v y). subst.
+  apply ALen_TFVar_I1. apply* binds_push_eq.
+  apply ALen_TFVar_I. auto_star.
+
+  inversion len; subst.
+  assert (v<>y). intros neq. subst. apply ok_push_inv in okg. destruct okg as [_ okg]. false binds_fresh_inv H1 okg.
+  apply ALen_EVar. apply* binds_concat_left.
   assert (v<>y). intros neq. subst. apply ok_push_inv in okg. destruct okg as [_ okg]. false okg. simpl_dom. apply union_left.  apply union_right. apply in_singleton_self.
   rewrite <- concat_assoc. apply* ALen_Solved_EVar.
   rewrite* concat_assoc.
-
+  assert (v<>y). intros neq. subst. apply ok_push_inv in okg. destruct okg as [_ okg]. false binds_fresh_inv H1 okg.
+  apply ALen_EVar_I1. apply* binds_concat_left.
+  assert (v<>y). intros neq. subst. apply ok_push_inv in okg. destruct okg as [_ okg]. false binds_fresh_inv H1 okg.
+  apply ALen_EVar_I2 with t. apply* binds_concat_left.
+  assert (v<>y). intros neq. subst. apply ok_push_inv in okg. destruct okg as [_ okg]. false binds_fresh_inv H1 okg.
+  apply ALen_EVar_I3. apply* binds_concat_left.
   destruct (eq_var_dec v y). subst.
   apply ALen_EVar_I1. apply* binds_push_eq.
-
   apply ALen_EVar_I. auto_star.
 
-  inversion len; subst. apply ALen_Star.
+  apply* alen_add_var_expr.
+Qed.
 
+Lemma alen_add_tvar_expr: forall G i y e,
+    ALen G (AT_Expr e) i ->
+    ok (G & y ~ AC_TVar) ->
+    ALen (G & y ~ AC_TVar) (AT_Expr e) i
+with alen_add_tvar: forall G i y e,
+    ALen G e i ->
+    ok (G & y ~ AC_TVar) ->
+    ALen (G & y ~ AC_TVar) e i.
+Proof.
+  introv len okg.
+  gen i. induction e; introv len.
+
+  inversion len; subst. apply ALen_BVar.
+
+  inversion len; subst.
+  assert (v<>y). intros neq. subst. apply ok_push_inv in okg. destruct okg as [_ okg]. false binds_fresh_inv H1 okg.
+  apply ALen_Var. apply* binds_concat_left.
+  assert (v<>y). intros neq. subst. apply ok_push_inv in okg. destruct okg as [_ okg]. false binds_fresh_inv H1 okg.
+  apply ALen_TypVar with t. apply* binds_concat_left.
+  assert (v<>y). intros neq. subst. apply ok_push_inv in okg. destruct okg as [_ okg]. false binds_fresh_inv H1 okg.
+  apply ALen_Var_I1. apply* binds_concat_left.
+  assert (v<>y). intros neq. subst. apply ok_push_inv in okg. destruct okg as [_ okg]. false binds_fresh_inv H1 okg.
+  apply ALen_Var_I2 with t. apply* binds_concat_left.
+  assert (v<>y). intros neq. subst. apply ok_push_inv in okg. destruct okg as [_ okg]. false binds_fresh_inv H1 okg.
+  apply ALen_Var_I3. apply* binds_concat_left.
+  destruct (eq_var_dec v y). subst.
+  apply ALen_Var_I3. apply* binds_push_eq.
+  apply ALen_Var_I. auto_star.
+
+  inversion len; subst. apply ALen_Star.
   inversion len; subst. apply ALen_App.
-  apply* IHe1. Omega.omega.
-  apply* IHe2. Omega.omega.
+  apply* IHe1.
+  apply* IHe2.
 
   inversion len; subst. apply ALen_Lam.
-  apply* IHe. Omega.omega.
+  apply* IHe.
 
   inversion len; subst. apply ALen_Pi.
-  apply* IHe1. Omega.omega.
-  apply* IHe2. Omega.omega.
-
-  inversion len; subst. apply ALen_Let.
-  apply* IHe1. Omega.omega.
-  apply* IHe2. Omega.omega.
+  apply* alen_add_tvar.
+  apply* alen_add_tvar.
 
   inversion len; subst. apply ALen_CastUp.
-  apply* IHe. Omega.omega.
+  apply* IHe.
 
   inversion len; subst. apply ALen_CastDn.
-  apply* IHe. Omega.omega.
+  apply* IHe.
 
   inversion len; subst. apply ALen_Ann.
-  apply* IHe1. Omega.omega.
-  apply* IHe2. Omega.omega.
-Qed.
+  apply* IHe.
+  apply* alen_add_tvar.
 
-Lemma alen_add_var: forall G e i y,
-    ALen G e i ->
-    ok (G & y ~ AC_Var) ->
-    ALen (G & y ~ AC_Var) e i.
+  inversion len; subst. apply ALen_Forall.
+  apply* alen_add_tvar.
 Proof.
-  introv len okg. apply* alen_add_var'.
+  introv len okg.
+  gen i. induction e; introv len.
+
+  inversion len; subst. apply ALen_TBVar.
+
+  inversion len; subst.
+  assert (v<>y). intros neq. subst. apply ok_push_inv in okg. destruct okg as [_ okg]. false binds_fresh_inv H1 okg.
+  apply ALen_TFVar. apply* binds_concat_left.
+  assert (v<>y). intros neq. subst. apply ok_push_inv in okg. destruct okg as [_ okg]. false binds_fresh_inv H1 okg.
+  apply ALen_TFVar_I1. apply* binds_concat_left.
+  assert (v<>y). intros neq. subst. apply ok_push_inv in okg. destruct okg as [_ okg]. false binds_fresh_inv H1 okg.
+  apply ALen_TFVar_I2 with t. apply* binds_concat_left.
+  assert (v<>y). intros neq. subst. apply ok_push_inv in okg. destruct okg as [_ okg]. false binds_fresh_inv H1 okg.
+  apply ALen_TFVar_I3. apply* binds_concat_left.
+  assert (v<>y). intros neq. subst. apply ok_push_inv in okg. destruct okg as [_ okg]. false binds_fresh_inv H1 okg.
+  apply ALen_TFVar_I4 with t. apply* binds_concat_left.
+  destruct (eq_var_dec v y). subst.
+  apply ALen_TFVar. apply* binds_push_eq.
+  apply ALen_TFVar_I. auto_star.
+
+  inversion len; subst.
+  assert (v<>y). intros neq. subst. apply ok_push_inv in okg. destruct okg as [_ okg]. false binds_fresh_inv H1 okg.
+  apply ALen_EVar. apply* binds_concat_left.
+  assert (v<>y). intros neq. subst. apply ok_push_inv in okg. destruct okg as [_ okg]. false okg. simpl_dom. apply union_left.  apply union_right. apply in_singleton_self.
+  rewrite <- concat_assoc. apply* ALen_Solved_EVar.
+  rewrite* concat_assoc.
+  assert (v<>y). intros neq. subst. apply ok_push_inv in okg. destruct okg as [_ okg]. false binds_fresh_inv H1 okg.
+  apply ALen_EVar_I1. apply* binds_concat_left.
+  assert (v<>y). intros neq. subst. apply ok_push_inv in okg. destruct okg as [_ okg]. false binds_fresh_inv H1 okg.
+  apply ALen_EVar_I2 with t. apply* binds_concat_left.
+  assert (v<>y). intros neq. subst. apply ok_push_inv in okg. destruct okg as [_ okg]. false binds_fresh_inv H1 okg.
+  apply ALen_EVar_I3. apply* binds_concat_left.
+  destruct (eq_var_dec v y). subst.
+  apply ALen_EVar_I3. apply* binds_push_eq.
+  apply ALen_EVar_I. auto_star.
+
+  apply* alen_add_tvar_expr.
 Qed.
 
-Lemma alen_open: forall G e i y,
+Lemma alen_open_expr: forall G e i y n,
+    ALen G (AT_Expr e) i ->
+    ok G ->
+    binds y AC_Var G ->
+    ALen G (AT_Expr (AOpenRec n (AE_FVar y) e)) i
+with alen_open: forall G e i y n,
     ALen G e i ->
     ok G ->
     binds y AC_Var G ->
-    ALen G (e @ y) i.
+    ALen G (AOpenTypRec n (AE_FVar y) e) i.
 Proof.
-  introv len okg bd. unfold AOpen.
-  gen i. generalize 0. induction e; introv len; unfold AOpen; simpls; try(solve[assumption]).
+  introv len okg bd.
+  gen i n. induction e; introv len; intro k; simpls; try(solve[assumption]).
 
-  case_if*. inversion len; subst. apply* ALen_Var.
+  simpls. auto. case_if*. inversion len; subst. apply* ALen_Var.
 
   inversion len; subst. apply ALen_App.
   apply* IHe1. apply* IHe2.
@@ -268,10 +397,8 @@ Proof.
   apply* IHe.
 
   inversion len; subst. apply ALen_Pi.
-  apply* IHe1. apply* IHe2.
-
-  inversion len; subst. apply ALen_Let.
-  apply* IHe1. apply* IHe2.
+  apply* alen_open.
+  apply* alen_open.
 
   inversion len; subst. apply ALen_CastUp.
   apply* IHe.
@@ -280,7 +407,59 @@ Proof.
   apply* IHe.
 
   inversion len; subst. apply ALen_Ann.
+  apply* IHe. apply* alen_open.
+
+  inversion len; subst. apply ALen_Forall.
+  apply* alen_open.
+Proof.
+  introv len okg bd.
+  gen i n. induction e; introv len; intro k; simpls; try(solve[assumption]).
+
+  simpls. auto.
+Qed.
+
+Lemma alen_topen_expr: forall G e i y n,
+    ALen G (AT_Expr e) i ->
+    ok G ->
+    binds y AC_TVar G ->
+    ALen G (AT_Expr (ATOpenRec n (AT_TFVar y) e)) i
+with alen_topen: forall G e i y n,
+    ALen G e i ->
+    ok G ->
+    binds y AC_TVar G ->
+    ALen G (ATOpenTypRec n (AT_TFVar y) e) i.
+Proof.
+  introv len okg bd.
+  gen i n. induction e; introv len; intro k; simpls; try(solve[assumption]).
+
+  inversion len; subst. apply ALen_App.
   apply* IHe1. apply* IHe2.
+
+  inversion len; subst. apply ALen_Lam.
+  apply* IHe.
+
+  inversion len; subst. apply ALen_Pi.
+  apply* alen_topen.
+  apply* alen_topen.
+
+  inversion len; subst. apply ALen_CastUp.
+  apply* IHe.
+
+  inversion len; subst. apply ALen_CastDn.
+  apply* IHe.
+
+  inversion len; subst. apply ALen_Ann.
+  apply* IHe. apply* alen_topen.
+
+  inversion len; subst. apply ALen_Forall.
+  apply* alen_topen.
+Proof.
+  introv len okg bd.
+  gen i n. induction e; introv len; intro k; simpls; try(solve[assumption]).
+
+  simpls. auto. case_if*. inversion len; subst. apply* ALen_TFVar.
+
+  simpls. auto.
 Qed.
 
 Lemma alen_awterm_append: forall G H e n,
@@ -293,25 +472,27 @@ Proof.
   induction len.
   auto.
   apply ALen_Var. apply* binds_concat_left_ok.
+  apply ALen_BVar.
   apply ALen_TypVar with t. apply* binds_concat_left_ok.
-  apply* ALen_LetVar. apply* binds_concat_left_ok. apply* IHlen. destruct (split_bind_context H0) as (G1 & G2 & Hg). rewrite Hg in wf.
-  assert (AWTerm G1 e).
-  rewrite <- concat_assoc in wf. apply AWf_left in wf. apply* awterm_bnd.
-  rewrite Hg. rewrite <- concat_assoc. apply* awterm_is_awterma. apply* awterm_weaken_ctx.
-  rewrite concat_assoc. apply AWf_left in wf. apply* awf_is_ok.
-
   apply* ALen_Var_I1. apply* binds_concat_left_ok.
   apply* ALen_Var_I2. apply* binds_concat_left_ok.
+  apply* ALen_Var_I3. apply* binds_concat_left_ok.
   inversion wt; subst; try(solve[false binds_fresh_inv H3 H0]).
 
   apply* ALen_EVar. apply* binds_concat_left_ok.
+  rewrite <- concat_assoc. apply* ALen_Solved_EVar.
+  rewrite* concat_assoc.
   apply* ALen_EVar_I1. apply* binds_concat_left_ok.
   apply* ALen_EVar_I2. apply* binds_concat_left_ok.
   apply* ALen_EVar_I3. apply* binds_concat_left_ok.
+  inversion wt; subst; try(solve[false binds_fresh_inv H3 H0]).
 
-  rewrite <- concat_assoc. apply* ALen_Solved_EVar.
-  rewrite* concat_assoc.
-
+  apply ALen_TBVar.
+  apply* ALen_TFVar. apply* binds_concat_left_ok.
+  apply* ALen_TFVar_I1. apply* binds_concat_left_ok.
+  apply* ALen_TFVar_I2. apply* binds_concat_left_ok.
+  apply* ALen_TFVar_I3. apply* binds_concat_left_ok.
+  apply* ALen_TFVar_I4. apply* binds_concat_left_ok.
   inversion wt; subst; try(solve[false binds_fresh_inv H3 H0]).
 
   apply* ALen_Star.
@@ -319,81 +500,71 @@ Proof.
   apply* ALen_App.
   inversion wt; subst. apply* ALen_Lam.
   inversion wt; subst. apply* ALen_Pi.
-  inversion wt; subst. apply* ALen_Let.
   inversion wt; subst. apply* ALen_CastUp.
   inversion wt; subst. apply* ALen_CastDn.
   inversion wt; subst. apply* ALen_Ann.
+  inversion wt; subst. apply* ALen_Forall.
 Qed.
 
-
-Lemma alen_exists': forall n G e,
+Lemma alen_exists': forall G e n,
     AWf G ->
     LibList.length G < n ->
+    AWTermA G e ->
     exists m, ALen G e m.
 Proof.
-  intro n. induction n as [|n']; introv okg len.
+  introv okg len wt. gen G e. induction n as [|n']; introv okg len wt.
   false. inversion len.
 
-    induction e.
+  induction wt.
   exists* 1.
-  assert ({v \in dom G}+{v \notin dom G}). apply* decidable_sumbool. apply indom_decidable.
-  destruct H as [hin | hnotin].
+  exists* 1.
+  assert ({x \in dom G}+{x \notin dom G}). apply* decidable_sumbool. apply indom_decidable.
+  destruct H0 as [hin | hnotin].
   (* in *)
-  assert (exists vx, binds v vx G) by apply* get_some.
-  destruct H as (vx & H). destruct vx; auto_star.
-  destruct (split_bind_context H) as (G1 & G2 & IG).
-  assert (exists n, ALen G1 a0 n). apply~ IHn'.
-
-    rewrite IG in okg. rewrite <- concat_assoc in okg. apply* AWf_left.
-
-  rewrite IG in len.
-  rewrite concat_def in len. repeat(rewrite LibList.length_app in len).
-    assert(LibList.length (v~ AC_Bnd a a0) = 1). rewrite single_def. rewrite LibList.length_cons. rewrite LibList.length_nil. Omega.omega.
-
-  Omega.omega.
-
-    destruct H0 as (n & H0). exists* (n + 1). apply ALen_LetVar with a a0; auto.
-
-  rewrite <- concat_assoc in IG. rewrite IG. apply* alen_awterm_append. rewrite* <- IG. apply awterm_is_awterma. rewrite IG in okg. rewrite concat_assoc in okg. apply AWf_left in okg. apply* awterm_bnd.
+  assert (exists vx, binds x vx G) by apply* get_some.
+  destruct H0 as (vx & H0). destruct vx; auto_star.
 
   (* notin *)
-
   exists* 1.
-
-  assert ({v \in dom G}+{v \notin dom G}). apply* decidable_sumbool. apply indom_decidable.
-  destruct H as [hin | hnotin].
+  exists* 1.
+  exists* 1.
+  exists* 1.
+  assert ({a \in dom G}+{a \notin dom G}). apply* decidable_sumbool. apply indom_decidable.
+  destruct H0 as [hin | hnotin].
   (* in *)
-  assert (exists vx, binds v vx G) by apply* get_some.
-  destruct H as (vx & H). destruct vx; auto_star.
+  assert (exists vx, binds a vx G) by apply* get_some.
+  destruct H0 as (vx & H0). destruct vx; try(solve[exists* 1]).
 
   destruct (split_bind_context H) as (G1 & G2 & IG).
-  assert (exists n, ALen G1 a n). apply~ IHn'.
+  assert (exists n, ALen G1 t n). apply~ IHn'.
   rewrite IG in okg. rewrite <- concat_assoc in okg. apply* AWf_left.
 
   rewrite IG in len.
   rewrite concat_def in len. repeat(rewrite LibList.length_app in len).
-  assert(LibList.length (v~ AC_Solved_EVar a) = 1). rewrite single_def. rewrite LibList.length_cons. rewrite LibList.length_nil. Omega.omega.
+  assert(LibList.length (a~ AC_Solved_EVar t) = 1). rewrite single_def. rewrite LibList.length_cons. rewrite LibList.length_nil. Omega.omega.
   Omega.omega.
-  destruct H0 as (ne & H0). exists (ne + 1). rewrite IG in *. apply ALen_Solved_EVar; auto.
+  apply awterm_is_awterma.
+  rewrite IG in okg. apply AWf_left in okg. apply awterm_solved_evar in okg. auto.
+  destruct H1 as (ne & H1). exists (ne + 1). rewrite IG in *. apply ALen_Solved_EVar; auto.
 
-  (* notin *)
+  exists* 1.
   exists* 1.
 
-  exists* 1.
-  destruct IHe1 as (n1 & IHe1). destruct IHe2 as (n2 & IHe2). exists* (n1 + n2 + 1).
-  destruct IHe as (n & IHe1). exists* (n + 1).
-  destruct IHe1 as (n1 & IHe1). destruct IHe2 as (n2 & IHe2). exists* (n1 + n2 + 1).
-  destruct IHe1 as (n1 & IHe1). destruct IHe2 as (n2 & IHe2). exists* (n1 + n2 + 1).
-  destruct IHe as (n & IHe1). exists* (n + 1).
-  destruct IHe as (n & IHe1). exists* (n + 1).
-  destruct IHe1 as (n1 & IHe1). destruct IHe2 as (n2 & IHe2). exists* (n1 + n2 + 1).
+  destruct IHwt1 as (n1 & IHe1); auto. destruct IHwt2 as (n2 & IHe2); auto. exists* (n1 + n2 + 1).
+  destruct IHwt as (n & IHe1); auto. exists* (n + 1).
+  destruct IHwt1 as (n1 & IHe1); auto. destruct IHwt2 as (n2 & IHe2); auto. exists* (n1 + n2 + 1).
+  destruct IHwt as (n & IHe1); auto. exists* (n + 1).
+  destruct IHwt as (n & IHe1); auto. exists* (n + 1).
+  destruct IHwt1 as (n1 & IHe1); auto. destruct IHwt2 as (n2 & IHe2); auto. exists* (n1 + n2 + 1).
+  destruct IHwt as (n & IHe1); auto. exists* (n + 1).
 Qed.
 
 Lemma alen_exists: forall G e,
     AWf G ->
+    AWTermA G e ->
     exists n, ALen G e n.
 Proof.
-  introv wf.
+  intros.
   apply* alen_exists'.
 Qed.
 
@@ -405,44 +576,42 @@ Proof.
   introv hy1. gen i2. induction hy1; introv hy2; inversion hy2; subst; auto;
   try(solve[apply (binds_func H) in H1; inversion H1]);
   try(solve[apply (binds_func H) in H2; inversion H2]).
-  lets: binds_func H H1. inversion H0; subst. lets: IHhy1 i0 H3. subst*.
-  false binds_fresh_inv H H2.
-  false binds_fresh_inv H1 H.
   apply binds_middle_eq_inv in H; auto. inversion H.
-  apply binds_middle_eq_inv in H; auto. inversion H.
-  apply binds_middle_eq_inv in H; auto. inversion H.
-  apply binds_middle_eq_inv in H; auto. inversion H.
-  apply binds_middle_eq_inv in H2; auto. inversion H2.
-  apply binds_middle_eq_inv in H2; auto. inversion H2.
-  apply binds_middle_eq_inv in H2; auto. inversion H2.
   apply binds_middle_eq_inv in H2; auto. inversion H2.
   apply ok_middle_eq2 in H0; auto.
   destruct H0 as [eqg [eqv eqg2]]. inversion eqv. subst. lets: IHhy1 i0 H3. subst*.
+  apply binds_middle_eq_inv in H2; auto. inversion H2.
+  apply binds_middle_eq_inv in H2; auto. inversion H2.
+  apply binds_middle_eq_inv in H2; auto. inversion H2.
   false H2. simpl_dom. apply union_left. apply union_right. apply in_singleton_self.
+  apply binds_middle_eq_inv in H; auto. inversion H.
+  apply binds_middle_eq_inv in H; auto. inversion H.
+  apply binds_middle_eq_inv in H; auto. inversion H.
   false H. simpl_dom. apply union_left. apply union_right. apply in_singleton_self.
 Qed.
 
 Lemma alen_evar: forall G1 G2 a t m n,
     ok (G1 & a ~ AC_Solved_EVar t & G2) ->
-    ALen (G1 & a ~ AC_Solved_EVar t & G2) (AE_EVar a) n ->
+    ALen (G1 & a ~ AC_Solved_EVar t & G2) (AT_EVar a) n ->
     ALen G1 t m ->
     n = m + 1.
 Proof.
   introv okg lena lent.
   inversion lena; subst.
   apply binds_middle_eq_inv in H1; auto. inversion H1.
-  apply binds_middle_eq_inv in H1; auto. inversion H1.
-  apply binds_middle_eq_inv in H1; auto. inversion H1.
-  apply binds_middle_eq_inv in H1; auto. inversion H1.
   apply ok_middle_eq2 in H; auto.
   destruct H as [eqg [eqv eqg2]]. inversion eqv. subst.
   lets: alen_eq H2 lent. subst*.
+  apply binds_middle_eq_inv in H1; auto. inversion H1.
+  apply binds_middle_eq_inv in H1; auto. inversion H1.
+  apply binds_middle_eq_inv in H1; auto. inversion H1.
   false H1. simpl_dom. apply union_left. apply union_right. apply in_singleton_self.
 Qed.
 
+Hint Resolve awterm_is_awterma.
 Theorem cpltctxsubst_exists': forall G e n m,
     AWf G ->
-    AWTerm G e ->
+    AWTermT G e ->
     n < m ->
     ALen G e n ->
     CompleteCtx G ->
@@ -453,47 +622,41 @@ Proof.
   inversion less.
 
   gen n. induction wt; introv less len; simpls; auto_star.
-  false (complete_contains_unsolved comp H).
 
-  destruct (split_bind_context H) as (G1 & G2 & HG). rewrite HG in *.
-  assert (exists e, ACpltCtxSubst G1 t e).
-     destruct(@alen_exists G1 t) as (nt & ex). do 2 apply* AWf_left.
-     apply IHm with nt; auto. do 2 apply* AWf_left. do 2 apply* complete_part_left. apply* awterm_solved_evar.
-     assert (ok (G1 & a ~ AC_Solved_EVar t & G2)). auto.
-     lets: alen_evar H0 len ex.  Omega.omega.
-
-  destruct H0 as (et & H0).
-  exists et. apply~ ACpltCtxSubst_EVar. do 2 apply* complete_part_left. apply* complete_part_right.
-
-  destruct(@alen_exists G e1) as (ne1 & ex1). auto. auto. assert (exists t1, ACpltCtxSubst G e1 t1). apply* IHm.
+  (* APP *)
+  destruct(@alen_exists G (AT_Expr e1)) as (ne1 & ex1). auto. auto. assert (exists t1, ACpltCtxSubst G (AT_Expr e1) t1). apply* IHm.
   inversion len; subst. lets: alen_eq H2 ex1. Omega.omega.
   destruct H as (t1 & Ht1).
-  destruct(@alen_exists G e2) as (ne2 & ex2). auto. auto.
-  assert (exists t2, ACpltCtxSubst G e2 t2). apply* IHm.
+  destruct(@alen_exists G (AT_Expr e2)) as (ne2 & ex2). auto. auto.
+  assert (exists t2, ACpltCtxSubst G (AT_Expr e2) t2). apply* IHm.
   inversion len; subst. lets: alen_eq H4 ex2. Omega.omega.
   destruct H as (t2 & Ht2).
-  exists* (DE_App t1 t2).
+  destruct t1 ; try(solve[inversion Ht1]).
+  destruct t2 ; try(solve[inversion Ht2]).
+  exists* (DT_Expr (DE_App d d0)).
 
+   (* LAM *)
   inversion len; subst.
   pick_fresh y.
   assert (IH1: y \notin L) by auto_star.
   assert (IH2: AWf (G & y ~ AC_Var)) by apply* AWf_Var.
-  assert (IH3: CompleteCtx (G & y ~ AC_Var)). unfold CompleteCtx. intros z zv bd eqzv. subst. apply binds_push_inv in bd. destruct bd as [[_ neq] | [_ neq]]. false neq. false complete_contains_unsolved comp neq.
-  assert (IH4: ALen (G & y ~ AC_Var) (e @ y) i).
+  assert (IH3: CompleteCtx (G & y ~ AC_Var)). apply* complete_add.
+  assert (IH4: ALen (G & y ~ AC_Var) (AT_Expr (e @ y)) i).
     apply alen_add_var with (y:=y) in H3.
-    apply* alen_open. apply* awf_is_ok.
+    apply* alen_open_expr. apply* awf_is_ok.
   assert (IH5: i < S m). Omega.omega.
   lets: H0 IH1 IH2 IH3 IH5 IH4.
   destruct H1 as (et & H1).
   apply* lam_solve.
 
+  (* Pi *)
   inversion len; subst.
   assert (IT1:  exists t, ACpltCtxSubst G t1 t). apply IHwt with (n:=i1); auto. Omega.omega.
   pick_fresh y.
   assert (IH1: y \notin L) by auto_star.
   assert (IH2: AWf (G & y ~ AC_Var)) by apply* AWf_Var.
-  assert (IH3: CompleteCtx (G & y ~ AC_Var)). unfold CompleteCtx. intros z zv bd eqzv. subst. apply binds_push_inv in bd. destruct bd as [[_ neq] | [_ neq]]. false neq. false complete_contains_unsolved comp neq.
-  assert (IH4: ALen (G & y ~ AC_Var) (t2 @ y) i2).
+  assert (IH3: CompleteCtx (G & y ~ AC_Var)). apply* complete_add.
+  assert (IH4: ALen (G & y ~ AC_Var) (t2 @' y) i2).
     apply alen_add_var with (y:=y) in H6.
     apply* alen_open. apply* awf_is_ok.
   assert (IH5: i2 < S m). Omega.omega.
@@ -502,78 +665,64 @@ Proof.
   destruct H1 as (et2 & H1).
   apply* pi_solve.
 
-  inversion len; subst.
-  assert (IT1:  exists t, ACpltCtxSubst G e1 t). apply IHwt with (n:=i1); auto. Omega.omega.
-  pick_fresh y.
-  assert (IH1: y \notin L) by auto_star.
-  assert (IH2: AWf (G & y ~ AC_Var)) by apply* AWf_Var.
-  assert (IH3: CompleteCtx (G & y ~ AC_Var)). apply* complete_add.
-  assert (IH4: ALen (G & y ~ AC_Var) (e2 @ y) i2).
-    apply alen_add_var with (y:=y) in H6.
-    apply* alen_open. apply* awf_is_ok.
-  assert (IH5: i2 < S m). Omega.omega.
-  lets: H0 IH1 IH2 IH3 IH5 IH4.
-  destruct IT1 as (et1 & IT1).
-  destruct H1 as (et2 & H1).
-  apply* let_solve.
-
-  assert (exists t, ACpltCtxSubst G e t).
-    destruct(@alen_exists G e) as (ne & ex). auto. auto. apply IHm with ne; auto.
+  (* CASTUP *)
+  assert (exists t, ACpltCtxSubst G (AT_Expr e) t).
+    destruct(@alen_exists G (AT_Expr e)) as (ne & ex). auto. auto. apply IHm with ne; auto.
   inversion len; subst. lets: alen_eq H1 ex. Omega.omega.
   destruct H as (et & H).
-  exists* (DE_CastUp et).
+  destruct et ; try(solve[inversion H]).
+  exists* (DT_Expr (DE_CastUp d)).
 
-  assert (exists t, ACpltCtxSubst G e t).
-    destruct(@alen_exists G e) as (ne & ex). auto. auto. apply IHm with ne; auto.
+  (* CASTDOWN *)
+  assert (exists t, ACpltCtxSubst G (AT_Expr e) t).
+    destruct(@alen_exists G (AT_Expr e)) as (ne & ex). auto. auto. apply IHm with ne; auto.
   inversion len; subst. lets: alen_eq H1 ex. Omega.omega.
   destruct H as (et & H).
-  exists* (DE_CastDn et).
+  destruct et ; try(solve[inversion H]).
+  exists* (DT_Expr (DE_CastDn d)).
 
-  destruct(@alen_exists G e1) as (ne1 & ex1). auto. auto. assert (exists t1, ACpltCtxSubst G e1 t1). apply* IHm.
+  (* ANN *)
+  destruct(@alen_exists G (AT_Expr e1)) as (ne1 & ex1). auto. auto. assert (exists t1, ACpltCtxSubst G (AT_Expr e1) t1). apply* IHm.
   inversion len; subst. lets: alen_eq H2 ex1. Omega.omega.
   destruct H as (t1 & Ht1).
   destruct(@alen_exists G e2) as (ne2 & ex2). auto. auto.
   assert (exists t2, ACpltCtxSubst G e2 t2). apply* IHm.
   inversion len; subst. lets: alen_eq H4 ex2. Omega.omega.
   destruct H as (t2 & Ht2).
-  exists* (DE_Ann t1 t2).
+  destruct t1 ; try(solve[inversion Ht1]).
+  exists* (DT_Expr (DE_Ann d t2)).
+
+  (* Forall *)
+  inversion len; subst.
+  pick_fresh y.
+  assert (IH1: y \notin L) by auto_star.
+  assert (IH2: AWf (G & y ~ AC_TVar)) by apply* AWf_TVar.
+  assert (IH3: CompleteCtx (G & y ~ AC_TVar)). apply* complete_add_tvar.
+  assert (IH4: ALen (G & y ~ AC_TVar) (s @#' y) i).
+    apply alen_add_tvar with (y:=y) in H3.
+    apply* alen_topen. apply* awf_is_ok.
+  assert (IH5: i < S m). Omega.omega.
+  lets: H0 IH1 IH2 IH3 IH5 IH4.
+  destruct H1 as (et2 & H1).
+  apply* forall_solve.
+
+  (* Unsolved_EVar *)
+  false (complete_contains_unsolved comp H).
+
+  (* Solved_EVar *)
+  destruct (split_bind_context H) as (G1 & G2 & HG). rewrite HG in *.
+  assert (exists e, ACpltCtxSubst G1 t e).
+     destruct(@alen_exists G1 t) as (nt & ex). do 2 apply* AWf_left.
+     apply awterm_is_awterma. apply* awterm_solved_evar.
+     apply IHm with nt; auto. do 2 apply* AWf_left. do 2 apply* complete_part_left. apply* awterm_solved_evar.
+     assert (ok (G1 & i ~ AC_Solved_EVar t & G2)). auto.
+     lets: alen_evar H0 len ex.  Omega.omega.
+  destruct H0 as (et & H0).
+  exists et. apply~ ACpltCtxSubst_EVar. do 2 apply* complete_part_left. apply* complete_part_right.
 Qed.
 
 Theorem cpltctxsubst_exists: cpltctxsubst_exists_def.
 Proof.
   introv. intros. destruct(@alen_exists G e) as (n & ex). auto. auto.
   apply* cpltctxsubst_exists'.
-Qed.
-
-Lemma complete_add_star: forall G x,
-    CompleteCtx G ->
-    CompleteCtx (G & x ~ AC_Typ AE_Star).
-Proof.
-  introv comp.
-  unfold CompleteCtx.
-  intros z zv bd eqzv. subst.
-  apply binds_push_inv in bd. destruct bd as [[_ neq] | [_ neq]].
-  false neq.
-  false complete_contains_unsolved comp neq.
-Qed.
-
-Theorem cpltctxtsubst_exists: cpltctxtsubst_exists_def.
-Proof.
-  introv wf wt comp.
-  induction wt.
-
-  pick_fresh y.
-  assert (IH1: y \notin L) by auto_star.
-  assert (IH2: AWf (G & y ~ AC_Typ AE_Star)). apply* AWf_TyVar.
-  apply AWf_Expr with (H := empty). apply* ATC_Sub.
-  rewrite subst_star. rewrite concat_empty_r. apply* AUnify_Star.
-  assert (IH3: CompleteCtx (G & y ~ AC_Typ AE_Star)). apply* complete_add_star.
-  lets: H0 IH1 IH2 IH3.
-  destruct H1 as (nt & H1).
-  apply* forall_solve.
-
-  lets: cpltctxsubst_exists wf H comp.
-  destruct H0 as (nt & H0).
-  exists* (DT_Expr nt).
-  apply* ACpltCtxTSubst_Expr.
 Qed.
